nlist lexicographic comparison

src/lowparse/LowParse.SteelST.VCList.Iterator.fsti
@@ -1,31 +1,11 @@
 module LowParse.SteelST.VCList.Iterator
 include LowParse.SteelST.VCList
-open Steel.ST.GenElim
-
+open Steel.ST.Util
 module AP = LowParse.SteelST.ArrayPtr
 
-let nlist_iterator_prop
+val nlist_iterator
   (#k: parser_kind)
-  (#t: Type)
-  (p: parser k t)
-  (n0: nat)
-  (va0: v (parse_nlist_kind n0 k) (nlist n0 t))
-  (a0: byte_array)
-  (n: nat)
-  (va: v (parse_nlist_kind n k) (nlist n t))
-  (nl: nat)
-  (vl: v (parse_nlist_kind nl k) (nlist nl t))
-: GTot prop
-=
-      k.parser_kind_subkind == Some ParserStrong /\
-      AP.merge_into (array_of vl) (array_of va) (array_of va0) /\
-      va0.contents == List.Tot.append vl.contents va.contents /\
-      n0 == nl + n
-
-[@@__reduce__]
-let nlist_iterator0
-  (#k: parser_kind)
-  (#t: Type)
+  (#t: Type0) // gen_elim universe issue
   (p: parser k t)
   (n0: nat)
   (va0: v (parse_nlist_kind n0 k) (nlist n0 t))
@@ -33,26 +13,8 @@ let nlist_iterator0
   (n: nat)
   (va: v (parse_nlist_kind n k) (nlist n t))
 : Tot vprop
-= exists_ (fun (nl: nat) -> exists_ (fun (vl: v (parse_nlist_kind nl k) (nlist nl t))  ->
-    aparse (parse_nlist nl p) a0 vl `star`
-    pure (nlist_iterator_prop p n0 va0 a0 n va nl vl)
-  ))
 
-let nlist_iterator
-  (#k: parser_kind)
-  (#t: Type)
-  (p: parser k t)
-  (n0: nat)
-  (va0: v (parse_nlist_kind n0 k) (nlist n0 t))
-  (a0: byte_array)
-  (n: nat)
-  (va: v (parse_nlist_kind n k) (nlist n t))
-: Tot vprop
-= nlist_iterator0 p n0 va0 a0 n va
-
-#set-options "--ide_id_info_off"
-
-let nlist_iterator_parser_kind
+val nlist_iterator_parser_kind
   (#opened: _)
   (#k: parser_kind)
   (#t: Type0) // gen_elim universe issue
@@ -69,17 +31,9 @@ let nlist_iterator_parser_kind
     (fun _ ->
       k.parser_kind_subkind == Some ParserStrong
     )
-= rewrite
-    (nlist_iterator p n0 va0 a0 n va)
-    (nlist_iterator0 p n0 va0 a0 n va);
-  let _ = gen_elim () in
-  noop ();
-  rewrite
-    (nlist_iterator0 p n0 va0 a0 n va)
-    (nlist_iterator p n0 va0 a0 n va)
 
 inline_for_extraction
-let nlist_iterator_begin
+val nlist_iterator_begin
   (#k: Ghost.erased parser_kind)
   (#t: Type)
   (p: parser k t)
@@ -97,19 +51,8 @@ let nlist_iterator_begin
     ))
     (k.parser_kind_subkind == Some ParserStrong)
     (fun _ -> True)
-= let _ = elim_aparse (parse_nlist n0 p) a0 in
-  let a = AP.split a0 0sz in
-  let _ = gen_elim () in
-  let _ = intro_nlist_nil (n0 - n0) p a0 in
-  let va = intro_aparse (parse_nlist n0 p) a in
-  rewrite
-    (nlist_iterator0 p n0 va0 a0 n0 va)
-    (nlist_iterator p n0 va0 a0 n0 va);
-  return a
 
-#push-options "--z3rlimit 16"
-
-let nlist_iterator_end
+val nlist_iterator_end
   (#opened: _)
   (#k: parser_kind)
   (#t: Type)
@@ -125,15 +68,8 @@ let nlist_iterator_end
       aparse (parse_nlist n p) a va)
     (fun _ ->
       aparse (parse_nlist n0 p) a0 va0)
-= rewrite
-    (nlist_iterator p n0 va0 a0 n va)
-    (nlist_iterator0 p n0 va0 a0 n va);
-  let _ = gen_elim () in
-  let _ = intro_nlist_sum n0 p _ a0 n a in
-  vpattern_rewrite (aparse _ _) va0
 
-#restart-solver
-let nlist_iterator_append
+val nlist_iterator_append
   (#opened: _)
   (#k: parser_kind)
   (#t: Type)
@@ -157,23 +93,8 @@ let nlist_iterator_append
       va.contents == va1.contents `List.Tot.append` va2.contents
     )
     (fun _ -> True)
-= List.Tot.append_length va1.contents va2.contents;
-  noop ();
-  rewrite
-    (nlist_iterator p n0 va0 a0 n va)
-    (nlist_iterator0 p n0 va0 a0 n va);
-  let _ = gen_elim () in
-  let vl = rewrite_aparse a0 (parse_nlist (n0 - n) p) in
-  List.Tot.append_assoc vl.contents va1.contents va2.contents;
-  noop ();
-  let _ = intro_nlist_sum (n0 - n2) p (n0 - n) a0 n1 a1 in
-  rewrite
-    (nlist_iterator0 p n0 va0 a0 n2 va2)
-    (nlist_iterator p n0 va0 a0 n2 va2)
 
-#pop-options
-
-let nlist_iterator_next
+val nlist_iterator_next
   (#opened: _)
   (#k: parser_kind)
   (#t: Type)
@@ -196,6 +117,3 @@ let nlist_iterator_next
       va.contents == va1.contents :: va2.contents
     )
     (fun _ -> True)
-= nlist_iterator_parser_kind p n0 va0 a0 n va;
-  let _ = intro_nlist_one p a1 1 in
-  nlist_iterator_append p a0 a1 va2
